new-backend/bvp_liveScript.sml
@@ -48,7 +48,7 @@ val pLive_def = Define `
      let (d1,l1) = pLive c1 (insert n1 () LN) in
      let (d2,l2) = pLive c2 live in
      let ns1' = inter ns1 l1 in
-     let ns2' = inter ns2 (delete n2 l2) in
+     let ns2' = inter ns2 (union (delete n1 live) (delete n2 l2)) in
        (Handle ns1' d1 n1 n2 ns2' d2, union ns1' ns2'))`;
 
 val state_rel_def = Define `
@@ -56,7 +56,7 @@ val state_rel_def = Define `
     s1.code = t1.code /\ s1.clock = t1.clock /\
     s1.globals = t1.globals /\ s1.space = t1.space /\
     s1.output = t1.output /\ s1.refs = t1.refs /\
-    s1.handler = t1.handler /\
+    s1.handler = t1.handler /\ (LENGTH s1.stack = LENGTH t1.stack) /\
     (!x. x IN domain live ==> (lookup x s1.locals = lookup x t1.locals))`;
 
 val state_rel_ID = prove(
@@ -72,14 +72,56 @@ val lookup_inter_domain = prove(
   ``x IN domain t2 ==> (lookup x (inter t1 t2) = lookup x t1)``,
   fs [lookup_inter,domain_lookup] \\ REPEAT BasicProvers.CASE_TAC);
 
+val pEval_NONE_jump_exc = prove(
+  ``(pEval (c,s) = (NONE,u1)) /\ (jump_exc u1 = SOME x) ==>
+    (jump_exc s = SOME (s with <| stack := x.stack ;
+                                  handler := x.handler ;
+                                  locals := x.locals |>))``,
+  REPEAT STRIP_TAC \\ MP_TAC (Q.SPECL [`c`,`s`] pEval_stack) \\ fs []
+  \\ fs [jump_exc_def] \\ REPEAT STRIP_TAC \\ fs []
+  \\ REPEAT (BasicProvers.FULL_CASE_TAC \\ fs [])
+  \\ SRW_TAC [] []);
+
+val pEval_NONE_jump_exc_ALT = prove(
+  ``(pEval (c,s) = (NONE,u1)) /\ (jump_exc s = SOME x) ==>
+    (jump_exc u1 = SOME (u1 with <| stack := x.stack ;
+                                  handler := x.handler ;
+                                  locals := x.locals |>))``,
+  REPEAT STRIP_TAC \\ MP_TAC (Q.SPECL [`c`,`s`] pEval_stack) \\ fs []
+  \\ fs [jump_exc_def] \\ REPEAT STRIP_TAC \\ fs []
+  \\ REPEAT (BasicProvers.FULL_CASE_TAC \\ fs [])
+  \\ SRW_TAC [] []);
+
+val jump_exc_IMP_state_rel = prove(
+  ``!s1 t1 s2 t2.
+      (jump_exc s1 = SOME s2) /\ (jump_exc t1 = SOME t2) /\
+      state_rel s1 t1 LN /\ (LENGTH s2.stack = LENGTH t2.stack) ==>
+      state_rel (s2 with handler := s1.handler)
+                (t2 with handler := t1.handler) LN``,
+  REPEAT STRIP_TAC
+  \\ FULL_SIMP_TAC std_ss [jump_exc_def]
+  \\ REPEAT (BasicProvers.FULL_CASE_TAC \\ fs [])
+  \\ SRW_TAC [] [] \\ fs [state_rel_def]);
+
+val LAST_N_LEMMA = prove(
+  ``(LAST_N (LENGTH xs + 1 + 1) (x::y::xs) = x::y::xs) /\
+    (LAST_N (LENGTH xs + 1) (x::xs) = x::xs)``,
+  MP_TAC (Q.SPEC `x::y::xs` LAST_N_LENGTH)
+  \\ MP_TAC (Q.SPEC `x::xs` LAST_N_LENGTH) \\ fs [ADD1]);
+
 val pEval_pLive = prove(
   ``!c s1 res s2 l2 t1 l1 d.
       (pEval (c,s1) = (res,s2)) /\ state_rel s1 t1 l1 /\
-      (pLive c l2 = (d,l1)) /\ (res <> SOME Error) ==>
+      (pLive c l2 = (d,l1)) /\ (res <> SOME Error) /\
+      (!s3. (jump_exc s1 = SOME s3) ==>
+            ?t3. (jump_exc t1 = SOME t3) /\ state_rel s3 t3 LN /\
+                 (t3.handler = s3.handler) /\
+                 (LENGTH t3.stack = LENGTH s3.stack)) ==>
       ?t2. (pEval (d,t1) = (res,t2)) /\
            state_rel s2 t2 (case res of
                             | NONE => l2
                             | _ => LN)``,
+
   ONCE_REWRITE_TAC [EQ_SYM_EQ]
   \\ recInduct pEval_ind \\ REPEAT STRIP_TAC
   THEN1 (* Skip *)
@@ -115,8 +157,8 @@ val pEval_pLive = prove(
     \\ Q.PAT_ASSUM `lookup n s.locals = lookup n t1.locals`
          (ASSUME_TAC o GSYM) \\ fs [get_var_def]
     \\ SRW_TAC [] [call_env_def]
-    \\ fs [jump_exc_def] \\ Cases_on `t1.handler < LENGTH t1.stack` \\ fs []
-    \\ cheat)
+    \\ Cases_on `jump_exc s` \\ fs [] \\ SRW_TAC [] []
+    \\ Cases_on `jump_exc t1` \\ fs [] \\ SRW_TAC [] [])
   THEN1 (* Return *)
    (fs [pEval_def,pLive_def] \\ Cases_on `get_var n s` \\ fs []
     \\ fs [state_rel_def]
@@ -129,15 +171,120 @@ val pEval_pLive = prove(
     \\ `?res2 u2. pEval (c2,u1) = (res2,u2)` by METIS_TAC [PAIR]
     \\ `?x2 l5. pLive c2 l2 = (x2,l5)` by METIS_TAC [PAIR]
     \\ `?x1 l6. pLive c1 l5 = (x1,l6)` by METIS_TAC [PAIR]
-    \\ fs [LET_DEF,pLive_def,pEval_def,PULL_FORALL,AND_IMP_INTRO]
+    \\ fs [LET_DEF,pLive_def,pEval_def]
     \\ FIRST_X_ASSUM (MP_TAC o GSYM o Q.SPECL [`l5`,`t1`]) \\ fs []
-    \\ FIRST_X_ASSUM (MP_TAC o GSYM o Q.SPECL [`l2`]) \\ fs []
-    \\ REPEAT STRIP_TAC
     \\ Cases_on `res1 = SOME Error` \\ fs []
-    \\ Cases_on `res1 = NONE` \\ fs [] \\ SRW_TAC [] []
-    THEN1 (FIRST_X_ASSUM (MP_TAC o GSYM o Q.SPECL [`t2`]) \\ fs [])
-    \\ fs [state_rel_def] \\ IMP_RES_TAC pEval_locals_LN \\ fs [])
-  THEN1 (* Handle *) cheat
+    \\ MATCH_MP_TAC IMP_IMP \\ STRIP_TAC THEN1 (METIS_TAC [])
+    \\ REPEAT STRIP_TAC
+    \\ REVERSE (Cases_on `res1 = NONE`) \\ fs []
+    THEN1 (SRW_TAC [] [] \\ Cases_on `res` \\ fs [])
+    \\ Q.PAT_ASSUM `!x y. bb` (MP_TAC o GSYM o Q.SPECL [`l2`,`t2`]) \\ fs []
+    \\ REV_FULL_SIMP_TAC std_ss []
+    \\ MATCH_MP_TAC IMP_IMP \\ REPEAT STRIP_TAC \\ fs []
+    \\ Q.PAT_ASSUM `!x.bbb` (ASSUME_TAC o GSYM)
+    \\ IMP_RES_TAC pEval_NONE_jump_exc \\ Q.PAT_ASSUM `!x.bbb` (K ALL_TAC)
+    \\ RES_TAC
+    \\ IMP_RES_TAC pEval_NONE_jump_exc_ALT \\ POP_ASSUM (K ALL_TAC)
+    \\ POP_ASSUM (K ALL_TAC) \\ fs []
+    \\ `state_rel u1 t2 LN` by fs [state_rel_def]
+    \\ MP_TAC (Q.SPECL [`u1`,`t2`] jump_exc_IMP_state_rel) \\ fs []
+    \\ ASM_SIMP_TAC (srw_ss()) [state_rel_def])
+  THEN1 (* Handle *)
+   (fs [pEval_def]
+    \\ Cases_on `cut_env ns1 s.locals` \\ fs []
+    \\ Q.MATCH_ASSUM_RENAME_TAC `cut_env ns1 s.locals = SOME env1` []
+    \\ Cases_on `cut_env ns2 s.locals` \\ fs []
+    \\ Q.MATCH_ASSUM_RENAME_TAC `cut_env ns2 s.locals = SOME env2` []
+    \\ Cases_on `pEval (c1,push_exc env1 env2 s)` \\ fs []
+    \\ Cases_on `pLive c1 (insert v () LN)` \\ fs [LET_DEF]
+    \\ Cases_on `pLive c2 l2` \\ fs []
+    \\ Q.MATCH_ASSUM_RENAME_TAC `pLive c2 l2 = (q2,r2)` []
+    \\ Q.MATCH_ASSUM_RENAME_TAC `pLive c1 (insert v () LN) = (q1,r1)` []
+    \\ fs [pLive_def,LET_DEF,pEval_def]
+    \\ `domain (inter ns1 r1) SUBSET domain t1.locals /\
+        domain (inter ns2 (delete n r2)) SUBSET domain t1.locals /\
+        domain (inter ns2 (union (delete v l2) (delete n r2))) SUBSET
+          domain t1.locals`
+           by ALL_TAC THEN1
+     (fs [domain_inter,SUBSET_DEF,cut_env_def,state_rel_def,
+          domain_union,domain_delete] \\ REPEAT STRIP_TAC
+      \\ RES_TAC \\ fs [domain_lookup])
+    \\ fs [cut_env_def]
+    \\ Q.ABBREV_TAC `ns3 = (inter ns1 r1)`
+    \\ Q.ABBREV_TAC `ns4 = (inter ns2 (union (delete v l2) (delete n r2)))`
+    \\ FIRST_X_ASSUM (MP_TAC o GSYM o Q.SPECL [`(insert v () LN)`,
+          `push_exc (inter t1.locals (ns3:num_set))
+                    (inter t1.locals (ns4:num_set)) t1`])
+    \\ fs [] \\ MATCH_MP_TAC IMP_IMP \\ STRIP_TAC THEN1
+     (REPEAT STRIP_TAC \\ UNABBREV_ALL_TAC \\ fs [] THEN1
+       (fs[state_rel_def,push_exc_def] \\ SRW_TAC [] []
+        \\ fs [lookup_inter_assoc,lookup_inter_domain]
+        \\ fs [domain_union,domain_inter,domain_delete]
+        \\ fs[lookup_inter]
+        \\ Cases_on `lookup x ns1` \\ fs []
+        THEN1 (REPEAT BasicProvers.CASE_TAC \\ fs [])
+        \\ fs [domain_lookup])
+      \\ fs [jump_exc_def,push_exc_def,LAST_N_LEMMA]
+      \\ SRW_TAC [] [] \\ fs [state_rel_def] \\ DECIDE_TAC)
+    \\ REPEAT STRIP_TAC \\ fs []
+    \\ Cases_on `q` \\ fs [] THEN1
+     (Cases_on `get_var v r` \\ Cases_on `pop_exc r` \\ fs []
+      \\ `get_var v t2 = SOME x` by (fs [state_rel_def,get_var_def] \\ NO_TAC)
+      \\ fs [] \\ (Q.SPECL [`q1`,`push_exc
+            (inter t1.locals (ns3:num_set))
+            (inter t1.locals (ns4:num_set)) t1`] pEval_stack |> MP_TAC) \\ fs []
+      \\ REPEAT STRIP_TAC
+      \\ ASM_SIMP_TAC (srw_ss()) [pop_exc_def,push_exc_def]
+      \\ fs [] \\ (Q.SPECL [`c1`,`push_exc env1 env2 s`]
+                     pEval_stack |> MP_TAC) \\ fs []
+      \\ REPEAT STRIP_TAC \\ fs [pop_exc_def,push_exc_def] \\ SRW_TAC [] []
+      \\ fs [state_rel_def,set_var_def,lookup_insert]
+      \\ REPEAT STRIP_TAC
+      \\ Q.MATCH_ASSUM_RENAME_TAC `x6 IN domain l2` []
+      \\ Cases_on `x6 = v` \\ fs []
+      \\ UNABBREV_ALL_TAC
+      \\ ASM_SIMP_TAC std_ss [lookup_inter,lookup_delete,lookup_union]
+      \\ `lookup x6 l2 = SOME ()` by fs [domain_lookup,oneTheory.one]
+      \\ fs [] \\ Cases_on `lookup x6 ns2` \\ fs []
+      THEN1 (REPEAT BasicProvers.CASE_TAC \\ fs [])
+      \\ fs [oneTheory.one]
+      \\ fs [domain_union,domain_inter,domain_delete]
+      \\ `x6 IN domain ns2` by METIS_TAC [domain_lookup]
+      \\ RES_TAC \\ fs [])
+    \\ Cases_on `x` \\ fs []
+    \\ Q.PAT_ASSUM `(res,s2) = xxx` (ASSUME_TAC o GSYM) \\ fs []
+    \\ FIRST_X_ASSUM MATCH_MP_TAC \\ fs [] \\ REPEAT STRIP_TAC
+    \\ (Q.SPECL [`q1`,`push_exc
+              (inter t1.locals (ns3:num_set))
+              (inter t1.locals (ns4:num_set)) t1`] pEval_stack |> MP_TAC) \\ fs []
+    \\ ASM_SIMP_TAC (srw_ss()) [Once jump_exc_def,push_exc_def,LAST_N_LEMMA]
+    \\ ONCE_REWRITE_TAC [EQ_SYM_EQ] \\ REPEAT STRIP_TAC
+    \\ fs [] \\ (Q.SPECL [`c1`,`push_exc env1 env2 s`]
+                    pEval_stack |> MP_TAC) \\ fs []
+    \\ ASM_SIMP_TAC (srw_ss()) [Once jump_exc_def,push_exc_def,LAST_N_LEMMA]
+    \\ ONCE_REWRITE_TAC [EQ_SYM_EQ] \\ REPEAT STRIP_TAC THEN1
+     (SRW_TAC [] [] \\ fs [state_rel_def,set_var_def,lookup_insert]
+      \\ REPEAT STRIP_TAC \\ Cases_on `x = n` \\ fs []
+      \\ Q.PAT_ASSUM `inter s.locals ns2 = r.locals` (ASSUME_TAC o GSYM)
+      \\ UNABBREV_ALL_TAC
+      \\ fs [] \\ ASM_SIMP_TAC std_ss [lookup_inter,lookup_delete,lookup_union]
+      \\ fs [domain_union,domain_inter,domain_delete]
+      \\ Cases_on `lookup x ns2` \\ fs []
+      THEN1 (REPEAT BasicProvers.CASE_TAC \\ fs [])
+      \\ `x IN domain ns2` by METIS_TAC [domain_lookup]
+      \\ `lookup x s.locals = lookup x t1.locals` by METIS_TAC []
+      \\ fs [] \\ fs [domain_lookup]
+      \\ REPEAT BasicProvers.CASE_TAC \\ fs [])
+    \\ fs [jump_exc_def,set_var_def]
+    \\ Cases_on `LAST_N (s.handler + 1) s.stack` \\ fs []
+    \\ Cases_on `t` \\ fs []
+    \\ Cases_on `h'` \\ fs []
+    \\ Cases_on `h` \\ fs [] \\ SRW_TAC [] []
+    \\ Cases_on `LAST_N (t1.handler + 1) t1.stack` \\ fs []
+    \\ Cases_on `t` \\ fs []
+    \\ Cases_on `h'` \\ fs []
+    \\ Cases_on `h` \\ fs [] \\ SRW_TAC [] []
+    \\ fs [state_rel_def])
   THEN1 (* If *) cheat
   THEN1 (* Call *) cheat);
 
@@ -156,12 +303,12 @@ val pLive_correct = prove(
   \\ fs [] \\ REPEAT STRIP_TAC
   \\ Cases_on `pEval (c,s)` \\ fs []
   \\ Cases_on `pEval (FST (pLive c LN),s)` \\ fs []
-  \\ SRW_TAC [] []
+  \\ SRW_TAC [] [] \\ Cases_on `q` \\ fs []
   \\ IMP_RES_TAC pEval_locals_LN
   \\ fs [state_rel_def,bvp_state_explode]
   \\ MP_TAC (Q.SPECL [`c`,`s`] pEval_stack)
   \\ MP_TAC (Q.SPECL [`FST (pLive c LN)`,`s`] pEval_stack)
-  \\ fs [] \\ Cases_on `q` \\ fs [] \\ Cases_on `x` \\ fs []
-  \\ REPEAT STRIP_TAC \\ fs [] \\ SRW_TAC [] [] \\ fs [] \\ cheat);
+  \\ fs [] \\ Cases_on `x` \\ fs []
+  \\ REPEAT STRIP_TAC \\ fs [] \\ SRW_TAC [] [] \\ fs []);
 
 val _ = export_theory();
